src/CFG/Collecting/LTR_Collect.thy
@@ -31,15 +31,15 @@ definition ltr_F :: "cfg \<Rightarrow> store set \<Rightarrow> ltr set \<Rightar
       {Root [(cfg_entry g, s)] | s. s \<in> S}
     \<union> {extend t (v, s') | t a v s'.
           t \<in> T \<and> (sink_node t, a, v) \<in> intra g \<and> edge_step a (sink_store t) = Some s'}
-    \<union> {Call caller [(FunctionEntry p, enter_state (sink_store caller))]
-          | caller dst args p cont.
-          caller \<in> T \<and> (sink_node caller, CallEdge dst args, FunctionEntry p, cont) \<in> calls g}
+    \<union> {Call caller [(FunctionEntry p, call_enter (CallEdge dst pars args) (sink_store caller))]
+          | caller dst pars args p cont.
+          caller \<in> T \<and> (sink_node caller, CallEdge dst pars args, FunctionEntry p, cont) \<in> calls g}
     \<union> {Resume caller callee
           (path caller @ [(cont, combine_collect dst (sink_store caller) (sink_store callee))])
-          | callee caller p dst args cont.
+          | callee caller p dst pars args cont.
           callee \<in> T \<and> caller_of callee = Some caller
           \<and> sink_node callee = FunctionResult p
-          \<and> (sink_node caller, CallEdge dst args, FunctionEntry p, cont) \<in> calls g}"
+          \<and> (sink_node caller, CallEdge dst pars args, FunctionEntry p, cont) \<in> calls g}"
 
 subsection \<open>Monotonicity\<close>
 
@@ -87,13 +87,13 @@ proof
       unfolding ltr_F_def[of g S "lfp (ltr_F g S)"] using intra.hyps intra.IH by blast
     then show ?case by (rule ltr_F_lfp_fold)
   next
-    case (call caller dst args p cont)
-    have "Call caller [(FunctionEntry p, enter_state (sink_store caller))]
+    case (call caller dst pars args p cont)
+    have "Call caller [(FunctionEntry p, call_enter (CallEdge dst pars args) (sink_store caller))]
             \<in> ltr_F g S (lfp (ltr_F g S))"
       unfolding ltr_F_def[of g S "lfp (ltr_F g S)"] using call.hyps call.IH by blast
     then show ?case by (rule ltr_F_lfp_fold)
   next
-    case (ret callee caller p dst args cont)
+    case (ret callee caller p dst pars args cont)
     have "Resume caller callee
             (path caller @ [(cont, combine_collect dst (sink_store caller) (sink_store callee))])
             \<in> ltr_F g S (lfp (ltr_F g S))"
@@ -170,12 +170,12 @@ text \<open>(3) Call entry: a collected call-site state produces the entered sta
   callee's \<^const>\<open>FunctionEntry\<close>.\<close>
 lemma ltr_collect_call:
   assumes "s \<in> ltr_collect g S u"
-    and "(u, CallEdge dst args, FunctionEntry p, cont) \<in> calls g"
-  shows "enter_state s \<in> ltr_collect g S (FunctionEntry p)"
+    and "(u, CallEdge dst pars args, FunctionEntry p, cont) \<in> calls g"
+  shows "call_enter (CallEdge dst pars args) s \<in> ltr_collect g S (FunctionEntry p)"
 proof -
   from assms(1) obtain t where t: "t \<in> valid_ltr g S" "sink_node t = u" "sink_store t = s"
     by (rule ltr_collect_E)
-  have "Call t [(FunctionEntry p, enter_state (sink_store t))] \<in> valid_ltr g S"
+  have "Call t [(FunctionEntry p, call_enter (CallEdge dst pars args) (sink_store t))] \<in> valid_ltr g S"
     by (rule valid_ltr.call[OF t(1)]) (use assms(2) t(2) in simp)
   from ltr_collect_I[OF this] show ?thesis using t(3) by simp
 qed
@@ -193,7 +193,7 @@ text \<open>(5) Resume: a collected completed callee activation produces the com
 lemma ltr_collect_resume:
   assumes "callee \<in> valid_ltr g S" and "caller_of callee = Some caller"
     and "sink_node callee = FunctionResult p"
-    and "(sink_node caller, CallEdge dst args, FunctionEntry p, cont) \<in> calls g"
+    and "(sink_node caller, CallEdge dst pars args, FunctionEntry p, cont) \<in> calls g"
   shows "combine_collect dst (sink_store caller) (sink_store callee) \<in> ltr_collect g S cont"
 proof -
   have "Resume caller callee
@@ -212,8 +212,8 @@ lemma ltr_collect_ctx_intra_pres:
 text \<open>(7) Context transition under call: the child activation receives exactly the context
   produced by the configured enter function.\<close>
 lemma ltr_collect_ctx_call:
-  "key enterc seedc (Call caller [(FunctionEntry p, enter_state (sink_store caller))])
-     = enterc (key enterc seedc caller) (enter_state (sink_store caller))"
+  "key enterc seedc (Call caller [(FunctionEntry p, call_enter (CallEdge dst pars args) (sink_store caller))])
+     = enterc (key enterc seedc caller) (call_enter (CallEdge dst pars args) (sink_store caller))"
   by simp
 
 text \<open>(8) Context restoration under resume: a resumed trace has the caller's activation
@@ -338,9 +338,9 @@ proof -
   have OUTER: "outer \<in> valid_ltr rec_cfg UNIV"
     unfolding outer_def by (rule valid_ltr.intra[OF R eA stepA])
   have so: "sink_node outer = Statement 1" by (simp add: outer_def)
-  have ecall: "(sink_node outer, CallEdge None [], FunctionEntry pr, Statement 200) \<in> calls rec_cfg"
+  have ecall: "(sink_node outer, CallEdge None [] [], FunctionEntry pr, Statement 200) \<in> calls rec_cfg"
     by (simp add: so rec_defs)
-  define inner where "inner = Call outer [(FunctionEntry pr, enter_state (sink_store outer))]"
+  define inner where "inner = Call outer [(FunctionEntry pr, call_enter (CallEdge None [] []) (sink_store outer))]"
   have INNER: "inner \<in> valid_ltr rec_cfg UNIV"
     unfolding inner_def by (rule valid_ltr.call[OF OUTER ecall])
   have neq: "outer \<noteq> inner" by (simp add: outer_def inner_def)
